src/Examples/QueryStructure/MessagesExtraction.v
@@ -35,7 +35,7 @@ Arguments ComputationalADT.pcConstructors / .
 Arguments callcADTMethod / .
 Arguments ComputationalADT.cMethods / .
 Arguments ComputationalADT.pcMethods / .
-Definition InitMessages : ComputationalADT.cRep MessagesImpl := Eval simpl in (CallConstructor MessagesImpl InitS tt).
+Definition InitMessages : ComputationalADT.cRep MessagesImpl := Eval simpl in (CallConstructor MessagesImpl InitS).
 (* currying functions (other fns take tuples) *)
 Definition AddMessage (num : nat) (time : nat) (msg : list string)
            (r : ComputationalADT.cRep MessagesImpl)
